Clean up.

Isabelle2/AbstractMultiPaxosR1Correctness.thy
@@ -49,35 +49,42 @@ method try_inv uses invs declares inv_defs =
       \<bar> R:"reachable ?ioa ?x" and P:"_"(multi) \<Rightarrow> 
         \<open>(insert P, instantiate_invs_2 invs:invs, try_ind_step) | print_term "''ind case failed''"\<close> )
     )
-  
+
+method inv_cases uses invs declares inv_defs =
+  (rule invariantI; (
+      ((match premises in "?s \<in> ioa.start ?ioa" \<Rightarrow> \<open>-\<close>))
+      | instantiate_invs_2 invs:invs; simp only:is_trans_simp;
+        ((induct_tac rule:trans_cases | print_term "''case analysis failed''"), simp?); rm_trans_rel_assm
+        ) )
+
 subsection {* Invariants *}
 
-definition inv7 where inv7_def[inv_defs]:
-  "inv7 s \<equiv> \<forall> a . ampr1_state.leader s a \<longrightarrow> leader (ballot s a) = a"
+definition inv1 where inv1_def[inv_defs]:
+  "inv1 s \<equiv> \<forall> a . ampr1_state.leader s a \<longrightarrow> leader (ballot s a) = a"
 
-lemma inv7: "invariant the_ioa inv7" by (try_inv)
+lemma inv1: "invariant the_ioa inv1" by (try_inv)
 
-definition inv6 where inv6_def[inv_defs]:
-  "inv6 s \<equiv> \<forall> a b i . leader b = a \<and> (ballot s a < b \<or> (ballot s a = b \<and> \<not> ampr1_state.leader s a))
+definition inv2 where inv2_def[inv_defs]:
+  "inv2 s \<equiv> \<forall> a b i . leader b = a \<and> (ballot s a < b \<or> (ballot s a = b \<and> \<not> ampr1_state.leader s a))
     \<longrightarrow> suggestion s i b = None"
 
-lemma inv6: "invariant the_ioa inv6"  by (try_inv invs:inv7)
+lemma inv2: "invariant the_ioa inv2"  by (try_inv invs:inv1)
 
-definition inv1 where inv1_def[inv_defs]:
+definition inv3 where inv3_def[inv_defs]:
   -- {* acceptors only vote for the suggestion. *}
-  "inv1 s \<equiv> \<forall> i a b . let v = vote s i a b in v \<noteq> None \<longrightarrow> v = suggestion s i b"
+  "inv3 s \<equiv> \<forall> i a b . let v = vote s i a b in v \<noteq> None \<longrightarrow> v = suggestion s i b"
 
-lemma inv1: "invariant the_ioa inv1"  by (try_inv invs:inv7 inv6)
+lemma inv3: "invariant the_ioa inv3"  by (try_inv invs:inv1 inv2)
 
 abbreviation conservative_array where
   "conservative_array s \<equiv>  \<forall> i . ballot_array.conservative_array (vote s i)"
 
 lemma conservative: "invariant the_ioa conservative_array"
 proof -
-  have "\<And> s . inv1 s \<Longrightarrow> conservative_array s"
+  have "\<And> s . inv3 s \<Longrightarrow> conservative_array s"
     apply (simp add:inv_defs ballot_array.conservative_def ballot_array.conservative_array_def
         split:option.splits) by (metis option.inject) 
-  with inv1 show ?thesis  using IOA.invariant_def by blast
+  with inv3 show ?thesis  using IOA.invariant_def by blast
 qed
 
 abbreviation safe_at where "safe_at s i \<equiv> ballot_array.safe_at quorums (ballot s) (vote s i)"
@@ -94,21 +101,37 @@ proof -
   by (metis ballot_array_prefix_axioms_def ballot_array_prefix_def quorums_axioms) 
 qed
 
-definition inv3 where inv3_def[inv_defs]:
-  "inv3 s \<equiv> \<forall> a b f i . onebs s a b = Some f \<longrightarrow> f i = dsa.acc_max (vote s i) a b \<and> ballot s a \<ge> b"
+context begin
+
+definition inv4 where inv4_def[inv_defs]:
+  "inv4 s \<equiv> \<forall> b i q . joined s q b \<and> q \<in> quorums \<longrightarrow> 
+  (case sugg s i b q of  Some v \<Rightarrow> dsa.proved_safe_at (ballot s) (vote s i) q b v
+  | None \<Rightarrow> (\<forall> v . dsa.proved_safe_at (ballot s) (vote s i) q b v))"
   
-lemma inv3: "invariant the_ioa inv3"
-  -- {* @{term inv3} is inductive on its own. The @{term do_vote} case necessitates  to show 
-  that the value of @{term dsa.acc_max} dose not change as a result of the vote. 
-  TODO: superseded by inv4. *}
-  apply try_inv
-  subgoal premises prems for s t _ a2 i2 v unfolding inv3_def
+text {* To show that @{term inv4} is invariant, we will use two auxiliary invariants. *}
+
+text {* First, we show that an acceptor that has sent a oneb for ballot b has indeed joined b, and that it includes
+  its maximum vote before b. *}
+
+definition inv4_1 where "inv4_1 s \<equiv> \<forall> a b f i . onebs s a b = Some f 
+      \<longrightarrow> f i = dsa.acc_max (vote s i) a b \<and> ballot s a \<ge> b"
+
+text {* Then, we show that @{term max_vote} is the maximum vote before b over a quorum that has joined b. *}
+
+definition inv4_2 where "inv4_2 s \<equiv> \<forall> i b q . joined s q b \<longrightarrow> 
+    (max_vote s i b q = dsa.max_quorum_votes (vote s i) q b) \<and> (\<forall> a \<in> q . ballot s a \<ge> b)"
+  
+private 
+lemma inv4_1:"invariant the_ioa inv4_1"
+  -- {* The @{term do_vote} case necessitates to show that the value of @{term dsa.acc_max} dose not change as a result of the vote.  *}
+  apply (try_inv inv_defs:inv4_1_def)
+  subgoal premises prems for s t _ a2 i2 v unfolding inv4_1_def
       -- {* the @{term do_vote} case *}
   proof (clarify, rule conjI)
     fix a b f i
     assume "onebs t a b = Some f"
     hence "onebs s a b = Some f" using \<open>do_vote a2 i2 v s t\<close> unfolding do_vote_def by auto
-    hence "f i = dsa.acc_max (vote s i) a b" and "b \<le> ballot s a" using \<open>inv3 s\<close> unfolding inv3_def by auto
+    hence "f i = dsa.acc_max (vote s i) a b" and "b \<le> ballot s a" using \<open>inv4_1 s\<close> unfolding inv4_1_def by auto
     have "dsa.acc_max (vote t i) a b = dsa.acc_max (vote s i) a b"
     proof -
       from \<open>b \<le> ballot s a\<close> have "\<And> b' . b' < b \<Longrightarrow> vote s i a b' = vote t i a b'" using  \<open>do_vote a2 i2 v s t\<close>
@@ -120,308 +143,149 @@ lemma inv3: "invariant the_ioa inv3"
     from \<open>b \<le> ballot s a\<close> and \<open>do_vote a2 i2 v s t\<close> show "b \<le> ballot t a" unfolding do_vote_def by auto
   qed
   done
-
-(* 
-method instantiate_inv uses inv = (
-  ( insert inv,
-    instantiate_invs )?,
-  match premises in R[thin]:"reachable ?ioa ?s" and T:"?s \<midarrow>?a\<midarrow>?ioa\<longrightarrow> ?t" \<Rightarrow> 
-    \<open>insert reachable_n[OF R T]\<close>,
-  ( insert inv,
-    instantiate_invs )?,
-  rm_reachable )
-*)
-
-definition inv4 where inv4_def[inv_defs]:
-  "inv4 s \<equiv> \<forall> i b q . joined s q b \<longrightarrow> 
-    (max_vote s i b q = dsa.max_quorum_votes (vote s i) q b) \<and> (\<forall> a \<in> q . ballot s a \<ge> b)"
-lemma inv4:"invariant the_ioa inv4"
-  -- {* This is a trivial consequence of @{thm inv3}. *}
+  
+private
+lemma inv4_2:"invariant the_ioa inv4_2"
 proof - 
-  have "inv4 s" if "inv3 s" for s unfolding inv4_def
+  have "inv4_2 s" if "inv4_1 s" for s unfolding inv4_2_def
   proof (clarsimp, rule conjI)
     fix i b q
     assume "joined s q b"
     hence "(the (onebs s a b)) i = dsa.acc_max (vote s i) a b" if "a \<in> q" for a
-      using \<open>inv3 s\<close> inv3_def joined_def that by fastforce
+      using \<open>inv4_1 s\<close> that by (simp add: ampr1_ioa.joined_def inv4_1_def) 
     thus "max_vote s i b q = dsa.max_quorum_votes (vote s i) q b" 
       unfolding max_vote_def dsa.max_quorum_votes_def by auto
-    show "\<forall>a\<in>q. b \<le> ballot s a" using \<open>inv3 s\<close> \<open>joined s q b\<close> unfolding joined_def inv3_def by auto
+    show "\<forall>a\<in>q. b \<le> ballot s a" using \<open>inv4_1 s\<close> \<open>joined s q b\<close> unfolding joined_def inv4_1_def by auto
   qed
-  thus ?thesis using IOA.invariant_def inv3 by blast 
+  thus ?thesis using IOA.invariant_def  inv4_1 by blast 
 qed
 
-definition inv15 where inv15_def[inv_defs]:
-  "inv15 s \<equiv> \<forall> b i q . joined s q b \<and> q \<in> quorums \<longrightarrow> 
-  (case sugg s i b q of  Some v \<Rightarrow> dsa.proved_safe_at (ballot s) (vote s i) q b v
-  | None \<Rightarrow> (\<forall> v . dsa.proved_safe_at (ballot s) (vote s i) q b v))"
-lemma inv15:"invariant the_ioa inv15"
-  -- {* Here the difficulty lies in the use of @{term the_elem} in @{thm sugg_def} *}
+lemma inv4:"invariant the_ioa inv4"
 proof -
-  have "inv15 s" if "inv4 s" and "conservative_array s" for s unfolding inv15_def
+  have "inv4 s" if "inv4_2 s" and "conservative_array s" for s unfolding inv4_def
   proof (clarify)
     fix b i q
     assume  "joined s q b" and "q \<in> quorums"
+    have "max_vote s i b q = dsa.max_quorum_votes (vote s i) q b" by (metis \<open>joined s q b\<close>  \<open>inv4_2 s\<close> inv4_2_def)
     let ?proved="dsa.proved_safe_at (ballot s) (vote s i) q b"
     show "case sugg s i b q of  Some v \<Rightarrow> ?proved v | None \<Rightarrow> (\<forall> v . ?proved v)"
     proof (cases "sugg s i b q")
       case None
-      then show ?thesis 
-          --  {* TODO*}
-        sorry
+      hence "dsa.max_quorum_votes (vote s i) q b = {}" unfolding sugg_def
+          \<open>max_vote s i b q = dsa.max_quorum_votes (vote s i) q b\<close> by auto
+      moreover from \<open>inv4_2 s\<close> and \<open>joined s q b\<close> have "\<And> a . a \<in> q \<Longrightarrow> ballot s a \<ge> b"
+        using inv4_2_def by blast 
+      ultimately show ?thesis using \<open>q \<in> quorums\<close> None unfolding dsa.proved_safe_at_def joined_def by auto 
     next
       case (Some v)
+        -- {* Here the difficulty lies in the use of @{term the_elem} in @{thm sugg_def} *}
       obtain x where "dsa.max_quorum_votes (vote s i) q b = {x}"
       proof -
         from Some have "max_vote s i b q \<noteq> {}" unfolding sugg_def by auto
         moreover
-        have "max_vote s i b q = dsa.max_quorum_votes (vote s i) q b" by (metis \<open>joined s q b\<close>  \<open>inv4 s\<close> inv4_def)
-        moreover 
-        have "ballot_array.conservative_array (vote s i)" using \<open>conservative_array s\<close> by auto
+        note \<open>max_vote s i b q = dsa.max_quorum_votes (vote s i) q b\<close>  and \<open>conservative_array s\<close> 
         moreover note dsa_p.max_vote_e_or_singleton
         ultimately show ?thesis using that  by (metis \<open>q \<in> quorums\<close>) 
       qed
       moreover 
-      have "v = (the_elem (fst ` (dsa.max_quorum_votes (vote s i) q b)))" using Some \<open>joined s q b\<close> \<open>inv4 s\<close>
-        by (auto simp add:inv4_def sugg_def)
-      ultimately show ?thesis using \<open>q\<in>quorums\<close> \<open>joined s q b\<close> \<open>inv4 s\<close> Some
-        unfolding dsa.proved_safe_at_def inv3_def inv4_def by auto
+      have "v = (the_elem (fst ` (dsa.max_quorum_votes (vote s i) q b)))" using Some \<open>joined s q b\<close> \<open>inv4_2 s\<close>
+        by (auto simp add:inv4_2_def sugg_def)
+      ultimately show ?thesis using \<open>q\<in>quorums\<close> \<open>joined s q b\<close> \<open>inv4_2 s\<close> Some
+        unfolding dsa.proved_safe_at_def inv4_2_def by auto
     qed
   qed
-  thus ?thesis by (metis (mono_tags, lifting) IOA.invariant_def conservative inv3 inv4)
+  thus ?thesis by (metis (mono_tags, lifting) IOA.invariant_def conservative inv4_2)
 qed
 
-definition inv12 where inv12_def[inv_defs]:
-  "inv12 s \<equiv> \<forall> b i q v . sugg s i b q = Some v \<and> joined s q b \<and> q \<in> quorums
-    \<longrightarrow> dsa.proved_safe_at (ballot s) (vote s i) q b v"
-lemma inv12:"invariant the_ioa inv12"
-  -- {* Here the difficulty lies in the use of @{term the_elem} in @{thm sugg_def} *}
-proof -
-  have "inv12 s" if "inv4 s" and "inv3 s" and "conservative_array s" for s unfolding inv12_def
-  proof  (clarify)
-    fix b i q v 
-    assume 1:"sugg s i b q = Some v" and 2:"joined s q b" and "q\<in>quorums"
-    obtain x where "dsa.max_quorum_votes (vote s i) q b = {x}"
-    proof -
-      from 1 have "max_vote s i b q \<noteq> {}" unfolding sugg_def by auto
-      moreover
-      have "max_vote s i b q = dsa.max_quorum_votes (vote s i) q b" by (metis "2" \<open>inv4 s\<close> inv4_def)
-      moreover 
-      have "ballot_array.conservative_array (vote s i)" using \<open>conservative_array s\<close> by auto
-      moreover note dsa_p.max_vote_e_or_singleton
-      ultimately show ?thesis using that by (metis \<open>q \<in> quorums\<close>) 
-    qed
-    moreover 
-    have "v = (the_elem (fst ` (dsa.max_quorum_votes (vote s i) q b)))" using 1 2 \<open>inv4 s\<close>
-      by (auto simp add:inv4_def sugg_def)
-    ultimately show "dsa.proved_safe_at (ballot s) (vote s i) q b v" using \<open>q\<in>quorums\<close> 2 \<open>inv3 s\<close>
-      unfolding dsa.proved_safe_at_def inv3_def joined_def
-      by (metis (full_types) image_empty image_insert insertI1 option.exhaust the_elem_eq)
-  qed
-  thus ?thesis by (metis (mono_tags, lifting) IOA.invariant_def conservative inv3 inv4)
-qed
+end
 
 abbreviation safe where "safe s \<equiv> \<forall> i . ballot_array.safe  quorums (ballot s) (vote s i)"
 declare ballot_array.safe_def[inv_defs]
 
-lemma aqcuire_leadership_ok:
+lemma aqcuire_leadership_safe:
   fixes a q s t i v safe_at 
   defines "safe_at w \<equiv> dsa.safe_at (ballot t) (vote t i) w (ballot t a)"
-  assumes "acquire_leadership a q s t" and "inv12 s" and "inv4 s" and "inv3 s" and "safe s"
-    and "conservative_array s"
+  assumes "acquire_leadership a q s t" and "inv4 s" and "safe s" and "conservative_array s"
   shows "case suggestion t i (ballot t a) of Some v \<Rightarrow> safe_at v | None \<Rightarrow> safe_at v"
+    -- {* Using @{thm inv4} and @{thm dsa_p.proved_safe_at_imp_safe_at}, we show that chaging leader is safe. *}
 proof -
-  let ?b = "ballot s a" 
-  have 3:"?b = ballot t a" using \<open>acquire_leadership a q s t\<close> by (auto simp add:inv_defs safe_at_def)
-  have 1:"q\<in>quorums" and 2:"\<And> a . a \<in> q \<Longrightarrow> ballot s a \<ge> ?b" using \<open>inv3 s\<close> \<open>acquire_leadership a q s t\<close> 
-    by (auto simp add:inv3_def) 
-  have 4:"vote s = vote t" and 5:"ballot s = ballot t" using \<open>acquire_leadership a q s t\<close> by auto
-  have 6:"suggestion t i ?b = sugg s i ?b q" using \<open>acquire_leadership a q s t\<close> by auto
+  let ?b = "ballot s a"
+  have 1:"q \<in> quorums" and 2:"joined s q ?b" using \<open>inv4 s\<close> \<open>acquire_leadership a q s t\<close> by (auto simp add:inv4_def) 
+  hence 3:"case sugg s i ?b q of None \<Rightarrow> \<forall>v. dsa.proved_safe_at (ballot s) (vote s i) q ?b v 
+    | Some v \<Rightarrow> dsa.proved_safe_at (ballot s) (vote s i) q ?b v" using \<open>inv4 s\<close> using inv4_def by blast 
+  have 4:"vote s = vote t" and 5:"ballot s = ballot t"
+    and 6:"suggestion t i ?b = sugg s i ?b q" using \<open>acquire_leadership a q s t\<close> by auto 
   show ?thesis
   proof (cases "suggestion t i ?b")
     case None
-    with 6 have 7:"sugg s i ?b q = None" by auto
-    have "dsa.proved_safe_at (ballot s) (vote s i) q ?b v"
-    proof -
-      have "max_vote s i ?b q = {}" using 7 by (auto simp add:sugg_def split!:if_splits) 
-      hence "dsa.max_quorum_votes (vote s i) q ?b = {}" using \<open>inv4 s\<close>
-        using assms(2) inv4_def by fastforce 
-      thus ?thesis using 1 2 by (auto simp add:dsa.proved_safe_at_def)
-    qed
-    with \<open>safe s\<close> and \<open>conservative_array s\<close> show ?thesis using 6 7 4 5 3 1
-      by (simp add: dsa_p.proved_safe_at_imp_safe_at safe_at_def)
+    with \<open>acquire_leadership a q s t\<close> have "sugg s i ?b q = None" by auto
+    with 3 have "dsa.proved_safe_at (ballot s) (vote s i) q ?b v" by simp 
+    thus ?thesis 
+      using "1" "4" "5" None assms(4) assms(5) dsa_p.proved_safe_at_imp_safe_at safe_at_def by fastforce 
   next
     case (Some w)
     from Some 6 have 7:"sugg s i ?b q = Some w" by auto
-    have "dsa.proved_safe_at (ballot s) (vote s i) q ?b w"
-    proof -
-      have "w = the_elem (fst ` (max_vote s i ?b q))" using 7 by (auto simp add:sugg_def split!:if_splits) 
-      hence "w = the_elem (fst ` (dsa.max_quorum_votes (vote s i) q ?b))" using \<open>inv4 s\<close>
-        using assms(2) by (auto simp add:inv4_def)
-      moreover obtain x where "dsa.max_quorum_votes (vote s i) q ?b = {x}" 
-      proof -
-        have "dsa.max_quorum_votes (vote s i) q ?b \<noteq> {}" using 7 \<open>inv4 s\<close> assms(2)
-          unfolding inv4_def by (simp add:sugg_def)
-        thus ?thesis using dsa_p.max_vote_e_or_singleton 1  \<open>conservative_array s\<close> that by blast
-      qed
-      ultimately show ?thesis using 1 2 by (simp add:dsa.proved_safe_at_def) 
-    qed
+    hence "dsa.proved_safe_at (ballot s) (vote s i) q ?b w" using "3" by auto 
     with \<open>safe s\<close> and \<open>conservative_array s\<close> show ?thesis using 6 7 4 5 3 1
       by (simp add: dsa_p.proved_safe_at_imp_safe_at safe_at_def)
   qed
 qed
 
-definition inv2 where
+definition inv5 where
   -- {* a suggestion is safe. *}
-  inv2_def[inv_defs]:
-  "inv2 s \<equiv> safe s \<and> (\<forall> i b . case suggestion s i b of Some v \<Rightarrow> safe_at s i v b 
-  | None \<Rightarrow> (ampr1_state.leader s (leader b) \<and> ballot s (leader b) = b) \<longrightarrow> (\<forall> v . safe_at s i v b))"
+  inv5_def[inv_defs]:
+  "inv5 s \<equiv> safe s 
+    \<and> (\<forall> i b . case suggestion s i b of Some v \<Rightarrow> safe_at s i v b 
+      | None \<Rightarrow> (ampr1_state.leader s (leader b) \<and> ballot s (leader b) = b) \<longrightarrow> (\<forall> v . safe_at s i v b))"
 
-lemma inv2:"invariant the_ioa inv2"
-  apply (rule invariantI)
-   apply (simp (no_asm_use) add:inv_defs ioa_defs split!:option.splits)
-   apply (simp add: dsa_p.safe_at_0)
-  subgoal premises prems for s t a
-  proof -
-    from prems(3) have 1:"\<And> i v b . safe_at s i v b \<Longrightarrow> safe_at t i v b" using safe_mono by auto
-    show ?thesis using prems
-      apply -
-      apply (instantiate_invs_2 invs:inv4 inv3 inv1 inv7 inv12 conservative)
-      apply (drule is_trans_E)
-      subgoal premises prems
-      proof -
-        have 2:?thesis if "suggestion t = suggestion s" and "ampr1_state.leader t = ampr1_state.leader s"
-          and "ballot t = ballot s" using that 1 \<open>inv1 t\<close> \<open>inv2 s\<close>
-          apply (auto simp add:inv_defs split:option.splits) apply metis by (metis option.distinct(1))
-        show ?thesis using prems
-          apply ((induct_tac rule:trans_cases, simp); rm_trans_rel_assm)
-          subgoal premises prems for c (* propose *)
-          proof -
-            show ?thesis using \<open>inv2 s\<close> \<open>propose c s t\<close> 
-              by (force simp add:inv_defs split!:option.splits) 
-          qed
-          subgoal premises prems for i v (* learn *)
-          proof -
-            show ?thesis using \<open>inv2 s\<close> \<open>learn i v s t\<close> by (simp add:inv_defs)
-          qed
-          subgoal premises prems for a b (* join_ballot *) 
-            using \<open>inv2 s\<close> \<open>join_ballot a b s t\<close> 1
-            apply (auto simp add:inv_defs split:option.splits)
-            by (metis option.distinct(1))
-          subgoal premises prems for a i v (* do_vote *)
-            using \<open>do_vote a i v s t\<close> 2 by simp
-          subgoal premises prems for a i b v (* suggest *)
-            apply (auto simp add:inv2_def split:option.split)
-            subgoal using \<open>suggest a i b v s t\<close> \<open>inv2 s\<close> by (simp add:inv2_def)
-            subgoal using \<open>suggest a i b v s t\<close> \<open>inv2 s\<close> by (force simp add:inv2_def split:option.splits)
-            subgoal premises prems2 for i2 b2 w
-            proof (cases "suggestion s i2 b2")
-              case None
-              then show ?thesis using \<open>suggest a i b v s t\<close> \<open>inv2 s\<close> prems2 \<open>inv7 s\<close>
-                apply (cases s, cases t, auto simp add:inv2_def inv7_def split:option.splits)
-                by (metis option.distinct(1))
-            next
-              case (Some v2)
-              then show ?thesis using \<open>suggest a i b v s t\<close> \<open>inv2 s\<close> prems2
-                by (simp add:inv2_def split:option.splits)
-            qed
-            done
-          subgoal premises prems for a q (* acquire_leadership *)
-          proof -
-            have "safe s" using \<open>inv2 s\<close> by (simp add:inv2_def)
-            have "leader (ballot t a) = a" and "q \<in> quorums" using \<open>acquire_leadership a q s t\<close> by auto
-            have "safe t" using \<open>inv2 s\<close> \<open>acquire_leadership a q s t\<close> by (auto simp add:inv2_def)
-            note 3 = aqcuire_leadership_ok[OF \<open>acquire_leadership a q s t\<close> \<open>inv12 s\<close> \<open>inv4 s\<close> \<open>inv3 s\<close> \<open>safe s\<close> \<open>conservative_array s\<close>]
-            show ?thesis using \<open>safe t\<close> 
-              apply (auto simp add:inv2_def split:option.splits)
-              subgoal premises prems2 for i2 b2 v2
-                apply (cases "b2 = ballot t a")
-                subgoal by (metis "3" option.case_eq_if \<open>suggestion t i2 b2 = None\<close>)
-                subgoal premises prems3 using \<open>acquire_leadership a q s t\<close> \<open>inv2 s\<close>
-                  apply (cases s, cases t, auto simp add:inv2_def split:option.splits)
-                  by (metis (no_types, lifting) ampr1_state.select_convs(2) ampr1_state.select_convs(4) ampr1_state.select_convs(6) fun_upd_apply option.distinct(1) prems2(2) prems2(3) prems2(4) prems3)
-                done
-              subgoal for i2 b2 x2 using 3 \<open>acquire_leadership a q s t\<close> \<open>inv2 s\<close> 
-                apply (cases s, cases t, auto simp add:inv2_def fun_upd_def split:option.splits)
-              proof -
-                fix propCmd :: "'b set" and ballota :: "'a \<Rightarrow> nat" and votea :: "nat \<Rightarrow> 'a \<Rightarrow> nat \<Rightarrow> 'b option" and suggestion :: "nat \<Rightarrow> nat \<Rightarrow> 'b option" and onebs :: "'a \<Rightarrow> nat \<Rightarrow> (nat \<Rightarrow> ('b \<times> nat) set) option" and leadera :: "'a \<Rightarrow> bool"
-                assume a1: "\<And>i v. case sugg \<lparr>propCmd = propCmd, ballot = ballota, vote = votea, suggestion = suggestion, onebs = onebs, leader = leadera\<rparr> i (ballota a) q of None \<Rightarrow> safe_at \<lparr>propCmd = propCmd, ballot = ballota, vote = votea, suggestion = \<lambda>i x. if x = ballota a then sugg \<lparr>propCmd = propCmd, ballot = ballota, vote = votea, suggestion = suggestion, onebs = onebs, leader = leadera\<rparr> i (ballota a) q else suggestion i x, onebs = onebs, leader = \<lambda>x. x = a \<or> leadera x\<rparr> i v (ballot \<lparr>propCmd = propCmd, ballot = ballota, vote = votea, suggestion = \<lambda>i x. if x = ballota a then sugg \<lparr>propCmd = propCmd, ballot = ballota, vote = votea, suggestion = suggestion, onebs = onebs, leader = leadera\<rparr> i (ballota a) q else suggestion i x, onebs = onebs, leader = \<lambda>x. x = a \<or> leadera x\<rparr> a) | Some v \<Rightarrow> safe_at \<lparr>propCmd = propCmd, ballot = ballota, vote = votea, suggestion = \<lambda>i x. if x = ballota a then sugg \<lparr>propCmd = propCmd, ballot = ballota, vote = votea, suggestion = suggestion, onebs = onebs, leader = leadera\<rparr> i (ballota a) q else suggestion i x, onebs = onebs, leader = \<lambda>x. x = a \<or> leadera x\<rparr> i v (ballot \<lparr>propCmd = propCmd, ballot = ballota, vote = votea, suggestion = \<lambda>i x. if x = ballota a then sugg \<lparr>propCmd = propCmd, ballot = ballota, vote = votea, suggestion = suggestion, onebs = onebs, leader = leadera\<rparr> i (ballota a) q else suggestion i x, onebs = onebs, leader = \<lambda>x. x = a \<or> leadera x\<rparr> a)"
-                assume "sugg \<lparr>propCmd = propCmd, ballot = ballota, vote = votea, suggestion = suggestion, onebs = onebs, leader = leadera\<rparr> i2 (ballota a) q = Some x2"
-                then have "(case Some x2 of None \<Rightarrow> dsa.safe_at ballota (votea i2) x2 (ballota a) | Some b \<Rightarrow> safe_at \<lparr>propCmd = propCmd, ballot = ballota, vote = votea, suggestion = \<lambda>n na. if na = ballota a then sugg \<lparr>propCmd = propCmd, ballot = ballota, vote = votea, suggestion = suggestion, onebs = onebs, leader = leadera\<rparr> n (ballota a) q else suggestion n na, onebs = onebs, leader = \<lambda>a. a = a \<or> leadera a\<rparr> i2 b (ballot \<lparr>propCmd = propCmd, ballot = ballota, vote = votea, suggestion = \<lambda>n na. if na = ballota a then sugg \<lparr>propCmd = propCmd, ballot = ballota, vote = votea, suggestion = suggestion, onebs = onebs, leader = leadera\<rparr> n (ballota a) q else suggestion n na, onebs = onebs, leader = \<lambda>a. a = a \<or> leadera a\<rparr> a)) = (case sugg \<lparr>propCmd = propCmd, ballot = ballota, vote = votea, suggestion = suggestion, onebs = onebs, leader = leadera\<rparr> i2 (ballota a) q of None \<Rightarrow> safe_at \<lparr>propCmd = propCmd, ballot = ballota, vote = votea, suggestion = \<lambda>n na. if na = ballota a then sugg \<lparr>propCmd = propCmd, ballot = ballota, vote = votea, suggestion = suggestion, onebs = onebs, leader = leadera\<rparr> n (ballota a) q else suggestion n na, onebs = onebs, leader = \<lambda>a. a = a \<or> leadera a\<rparr> i2 x2 (ballot \<lparr>propCmd = propCmd, ballot = ballota, vote = votea, suggestion = \<lambda>n na. if na = ballota a then sugg \<lparr>propCmd = propCmd, ballot = ballota, vote = votea, suggestion = suggestion, onebs = onebs, leader = leadera\<rparr> n (ballota a) q else suggestion n na, onebs = onebs, leader = \<lambda>a. a = a \<or> leadera a\<rparr> a) | Some b \<Rightarrow> safe_at \<lparr>propCmd = propCmd, ballot = ballota, vote = votea, suggestion = \<lambda>n na. if na = ballota a then sugg \<lparr>propCmd = propCmd, ballot = ballota, vote = votea, suggestion = suggestion, onebs = onebs, leader = leadera\<rparr> n (ballota a) q else suggestion n na, onebs = onebs, leader = \<lambda>a. a = a \<or> leadera a\<rparr> i2 b (ballot \<lparr>propCmd = propCmd, ballot = ballota, vote = votea, suggestion = \<lambda>n na. if na = ballota a then sugg \<lparr>propCmd = propCmd, ballot = ballota, vote = votea, suggestion = suggestion, onebs = onebs, leader = leadera\<rparr> n (ballota a) q else suggestion n na, onebs = onebs, leader = \<lambda>a. a = a \<or> leadera a\<rparr> a))"
-                  by simp
-                then show "dsa.safe_at ballota (votea i2) x2 (ballota a)"
-                  using a1
-                  by (smt \<open>sugg \<lparr>propCmd = propCmd, ballot = ballota, vote = votea, suggestion = suggestion, onebs = onebs, leader = leadera\<rparr> i2 (ballota a) q = Some x2\<close> ampr1_state.select_convs(2) ampr1_state.select_convs(3) option.simps(5)) 
-              qed
-              done
-          qed
-          done
-      qed
-      done
+method insert_safe_mono = 
+  match premises in P:"?s \<midarrow>?a\<midarrow>the_ioa\<longrightarrow> ?t" \<Rightarrow> \<open>insert safe_mono[OF P]\<close>
+
+method inv_cases_2 uses invs declares inv_defs =
+  (rule invariantI; (
+      ((match premises in "?s \<in> ioa.start ?ioa" \<Rightarrow> \<open>-\<close>))
+      | instantiate_invs_2 invs:invs; insert_safe_mono, simp only:is_trans_simp;
+        ((induct_tac rule:trans_cases | print_term "''case analysis failed''"), simp?); rm_trans_rel_assm
+        ) )
+
+lemma inv5:"invariant the_ioa inv5"
+  apply (inv_cases_2 invs:inv4 inv3 inv1 conservative)
+        apply (simp (no_asm_use) add:inv_defs ioa_defs split!:option.splits, simp add: dsa_p.safe_at_0) (* base case *)
+       apply (force simp add:inv5_def split:option.splits) (* propose *)
+      apply (force simp add:inv_defs split:option.splits) (* learn *)
+     apply (simp add:inv_defs split:option.splits; metis option.distinct(1)) (* join_ballot *)
+  subgoal premises prems for s t _ a i v unfolding inv5_def (* do_vote *)
+  proof (rule conjI)
+    note mono = \<open>\<And>i v b. safe_at s i v b \<Longrightarrow> safe_at t i v b\<close>
+    from \<open>do_vote a i v s t\<close> have "suggestion t = suggestion s" and "ampr1_state.leader t = ampr1_state.leader  s" and "ballot t = ballot s" by auto
+    with \<open>inv5 s\<close> and mono show " \<forall>i b. case suggestion t i b of None \<Rightarrow>
+      ampr1_state.leader t (leader b) \<and> ballot t (leader b) = b \<longrightarrow> (\<forall>v. safe_at t i v b)
+      | Some v \<Rightarrow> safe_at t i v b" apply (auto simp add:inv5_def split:option.splits) by (metis option.distinct(1))
+    show "safe t" using mono \<open>inv5 s\<close> \<open>inv3 t\<close> \<open>suggestion t = suggestion s\<close> by (auto simp add:inv3_def inv5_def dsa.safe_def split:option.splits; metis)
+  qed
+   apply (simp add:inv_defs split:option.splits; metis option.distinct(1)) (* suggest *)
+  subgoal premises prems for s t _ a q unfolding inv5_def (* acquire_leadership *)
+  proof (rule conjI)
+    note mono = \<open>\<And>i v b. safe_at s i v b \<Longrightarrow> safe_at t i v b\<close>
+    show "safe t" using \<open>inv5 s\<close> mono and \<open>acquire_leadership a q s t\<close> by (simp add:inv5_def)
+    have "safe s" using inv5_def \<open>inv5 s\<close> by blast
+    note aqcuire_leadership_safe[OF \<open>acquire_leadership a q s t\<close> \<open>inv4 s\<close> \<open>safe s\<close> \<open>conservative_array s\<close>]
+    moreover have "ballot t = ballot s" and "vote t = vote s" 
+      and "\<And> b i . b \<noteq> ballot s a \<Longrightarrow> suggestion t i b = suggestion s i b" 
+      and "ampr1_state.leader t = (ampr1_state.leader s)(a := True)" using \<open>acquire_leadership a q s t\<close> by simp_all
+    ultimately show " \<forall>i b. case suggestion t i b of None \<Rightarrow>
+      ampr1_state.leader t (leader b) \<and> ballot t (leader b) = b \<longrightarrow> (\<forall>v. safe_at t i v b)
+      | Some v \<Rightarrow> safe_at t i v b" using mono \<open>inv5 s\<close> \<open>inv1 s\<close> mono
+      apply (simp add:inv5_def inv1_def split:option.splits)
+      by (metis (no_types, lifting) option.case_eq_if option.distinct(1) option.sel)
   qed
   done
-declare inv2[invs]
 
-definition inv9 where
-  inv9_def[inv_defs]:"inv9 s \<equiv> \<forall> i a b . ballot s a < b \<longrightarrow> vote s i a b = None"
+definition inv6 where
+  inv6_def[inv_defs]:"inv6 s \<equiv> \<forall> i a b . ballot s a < b \<longrightarrow> vote s i a b = None"
 
-lemma  inv9:"invariant the_ioa inv9"
-apply (rule invariantI)
-apply (force simp add:inv_defs ioa_defs)
-  apply (unfold_to_trans_rel)
-  apply ((induct_tac rule:trans_cases, simp); rm_reachable; rm_trans_rel_assm;
-      (simp add:inv_defs; fail)?)
-done
-declare inv9[invs]
-
-lemma chosen_mono: assumes "chosen s i v" and "s \<midarrow>a\<midarrow>the_ioa\<longrightarrow> t"
-  shows "chosen t i v" using assms
-apply (unfold_to_trans_rel)
-apply ((induct_tac rule:trans_cases, simp); rm_trans_rel_assm)
-apply (auto simp add:inv_defs split:option.splits)[3] defer
-apply (auto simp add:inv_defs split:option.splits)[1]
-apply (cases s, cases t, auto simp add:inv_defs ballot_array.chosen_def ballot_array.chosen_at_def split:option.splits)
-  by (metis option.distinct(1))
-
-(*
-definition inv10 where inv4_def[inv_defs]:
-  "inv10 s \<equiv> \<forall> i l . case learned s l i of Some v \<Rightarrow> chosen s i v | None \<Rightarrow> True"
-
-lemma  inv10:"invariant the_ioa inv4"
-apply (rule invariantI)
-apply (force simp add:inv_defs)
-apply instantiate_invs_2
-apply (unfold_to_trans_rel)
-apply (induct_tac rule:trans_cases, simp)
-apply (auto simp add:inv_defs split:option.splits)[3] defer
-apply (auto simp add:inv_defs split:option.splits)[1]
-apply (insert chosen_mono[simplified inv_defs])
-apply (auto simp add:inv4_def inv5_def  split:option.splits) oops
-by (metis (mono_tags) ampr1_state.select_convs(3) ampr1_state.surjective ampr1_state.update_convs(3) fun_upd_same)
-declare inv4[invs]
-
-
-subsection {* Finally, the proof of agreement. *}
-
-definition agreement where agreement_def[inv_defs]:
-  "agreement s \<equiv> \<forall> i l1 l2 . let v = learned s l1 i; w = learned s l2 i 
-    in v \<noteq> None \<and> w \<noteq> None \<longrightarrow> v = w"
-
-lemma agreement:"invariant the_ioa agreement"
-proof -
-  text {* We prove that @{term inv4} and @{term  safe} imply @{term agreement}. 
-    Therefore, since they are invariant, @{term agreement} is invariant} *}
-  have "agreement s" if "inv4 s" and "safe s" for s
-  proof (auto simp add:inv_defs)
-    fix i l1 l2 v w
-    assume a1:"learned s l1 i = Some v" and a2:"learned s l2 i = Some w"
-    with \<open>inv4 s\<close> have "chosen s i v" and "chosen s i w" by (auto simp add:inv_defs split:option.splits)
-    with \<open>safe s\<close> show "v = w" by (metis ballot_array_props.intro ballot_array_props.safe_imp_agreement quorums_axioms)
-  qed
-  thus ?thesis using inv4 inv8_inv2_safe oops by (metis (mono_tags, lifting) IOA.invariant_def)
-qed
-    
-*)
+lemma  inv6:"invariant the_ioa inv6"
+by (try_inv)
 
 end
 
